Proved ARRAY

theories/clang/lib/array.v
@@ -38,6 +38,19 @@ Section array.
        | _, _ => False%I
      end)%I.
 
+  Lemma comm_assoc_s x y: x + S y = S x + y. Proof. omega. Qed.
+  Lemma assoc_s x y: S (x + y) = S x + y. Proof. omega. Qed.
+  Lemma distri_one x i: x + x * i = x * (i + 1).
+  Proof.
+    rewrite Nat.mul_add_distr_l Nat.mul_1_r. omega.
+  Qed.
+
+  Ltac assoc_nat :=
+    match goal with
+      | |- context [ ?E + (?E1 + ?E2) ] => replace (E + (E1 + E2)) with (E + E1 + E2); last omega
+      | |- context [ ?E + ?E1 + ?E2 ] => replace (E + E1 + E2) with (E + (E1 + E2)); last omega
+    end.
+  
   Lemma split_slice q t b o:
     ∀ l1 i l2 vs1 vs2,
       slice q t b o i l1 vs1 ∗ slice q t b o (i + l1) l2 vs2 ⊣⊢
@@ -56,30 +69,41 @@ Section array.
       + iIntros "[Hs1 Hs2]".
         destruct vs1=>//; simpl; first by iDestruct "Hs1" as "%".
         iDestruct "Hs1" as "[Hv Hl1']".
-        iFrame.
-        replace (i + S l1') with (S i + l1')=>//; last omega.
+        iFrame. rewrite comm_assoc_s.
         iAssert (⌜length vs1 = l1'⌝ ∗ slice q t b o (S i) (l1' + l2) (vs1 ++ vs2))%I with "[-]" as "[% ?]".
         { iApply IHl1'. iFrame. }
         iFrame. by subst.
       + iIntros "[% Hs]".
         simpl. destruct vs1=>//; simpl in *.
         simplify_eq.
-        iDestruct "Hs" as "[? ?]". iFrame.
-        replace (i + S (length vs1)) with (S i + length vs1)=>//; last omega.
+        iDestruct "Hs" as "[? ?]". iFrame. rewrite comm_assoc_s.
         iApply IHl1'.
         iSplit=>//.
   Qed.
 
-  Definition slice' q p t i l vs := let '(b, o) := p in slice q t b o i l vs.
-
-  Definition split_slice' q t p i l1 l2 vs1 vs2:
-    slice' q p t i l1 vs1 ∗ slice' q p t (i + l1) l2 vs2 ⊣⊢
-    ⌜ length vs1 = l1 ⌝ ∗ slice' q p t i (l1 + l2) (vs1 ++ vs2).
+  Lemma split_slice_join q t b o l1 i l2 vs1 vs2:
+    slice q t b o i l1 vs1 ∗ slice q t b o (i + l1) l2 vs2 ⊢
+    slice q t b o i (l1 + l2) (vs1 ++ vs2).
+  Proof. iIntros "~". by iDestruct (split_slice with "~") as "[_ ?]". Qed.
+  
+  Lemma split_slice' q t b o k n vs:
+    k < n → length vs = n →
+    slice q t b o 0 k (take k vs) ∗ slice q t b o k (n - k) (drop k vs) ⊣⊢
+    slice q t b o 0 n vs.
   Proof.
-    destruct p. iSplit.
-    - iIntros "[? ?]". iApply split_slice; iFrame.
-    - iIntros "?". iApply split_slice; iFrame.
+    intros ??.
+    rewrite -{3}(take_drop k vs).
+    assert (n = k + (n - k)) as H2; first omega.
+    rewrite {2}H2.
+    assert (k = 0 + k) as H3; first omega.
+    rewrite {3}H3.
+    iSplit.
+    - iIntros "?". by iDestruct (split_slice with "~") as "[% ?]".
+    - iIntros "?". iApply split_slice. iFrame.
+      iPureIntro. apply take_length_le. rewrite H1. omega.
   Qed.
+  
+  Definition slice' q p t i l vs := let '(b, o) := p in slice q t b o i l vs.
 
   Definition single_slice q b o t i v:
     slice q t b o i 1 [v] ⊣⊢ (b, o + sizeof t * i) ↦{q} v @ t.
@@ -96,18 +120,11 @@ Section array.
   Proof.
     induction vs as [|v' vs' IHvs'].
     - iIntros (???). iSplit; iIntros "?"; destruct l=>//.
-    - iIntros (???). iSplit; iIntros "?"; destruct l=>//; simpl.
-      + replace (o + sizeof_type t * (i + 1)) with (o + sizeof_type t + sizeof_type t * i).
-        iDestruct "~" as "[? ?]". iFrame.
-        replace (S (i + 1)) with (S i + 1). by iApply IHvs'.
-        { omega. }
-        { rewrite Nat.mul_add_distr_l -assoc Nat.mul_1_r. omega. }
-      + replace (o + sizeof_type t * (i + 1)) with (o + sizeof_type t + sizeof_type t * i).
-        iDestruct "~" as "[? ?]". iFrame.
-        replace (S (i + 1)) with (S i + 1). by iApply IHvs'.
-        { omega. }
-        { rewrite Nat.mul_add_distr_l -assoc Nat.mul_1_r. omega. }
-  Qed. (* FIXME: verbose *)
+    - iIntros (???).
+      iSplit; iIntros "?"; destruct l=>//; simpl;
+      rewrite assoc_s -distri_one; assoc_nat;
+      iDestruct "~" as "[? ?]"; iFrame; by iApply IHvs'.
+  Qed.
 
   Definition array_slice q t: ∀ n vs b o i,
     (b, o + sizeof_type t * i) ↦{q} varray vs @ tyarray t n ⊣⊢ slice q t b o i n vs.
@@ -132,26 +149,48 @@ Section array.
         iFrame. simpl.
         replace (o + sizeof_type t * i + sizeof_type t) with (o + sizeof_type t * S i).
         iDestruct (IHn' with "H2") as "?". done.
-        admit.
+        { replace (S i) with (i + 1); last omega.
+          rewrite -distri_one. omega. }
       + iIntros "Hs". simpl.
         destruct vs=>//; first by iDestruct "Hs" as "%".
         simpl. iApply mapstoval_join. iDestruct "Hs" as "[? ?]".
         iFrame. simpl.
         replace (o + sizeof_type t * i + sizeof_type t) with (o + sizeof_type t * S i).
         by iApply IHn'.
-        admit.
-  Admitted.
+        { replace (S i) with (i + 1); last omega.
+          rewrite -distri_one. omega. }
+  Qed.
 
   Lemma array_slice' q t n vs b o:
     (b, o) ↦{q} varray vs @ tyarray t n ⊣⊢ slice q t b o 0 n vs.
-  Proof. Admitted.
+  Proof. assert (o = o + sizeof_type t * 0) as Ho.
+         { rewrite Nat.mul_0_r Nat.add_0_r. done. }
+         rewrite {1}Ho.
+         apply array_slice. Qed.
 
-  Lemma index_spec q t p i n vs Φ:
-    i < n →
+  Lemma len_slice q t b o n vs:
+    slice q t b o 0 n vs ⊢ ⌜ length vs = n ⌝.
+  Proof.
+    iIntros "?". iDestruct (array_slice' with "~") as "~".
+    iDestruct (mapsto_typeof with "~") as "%".
+    iPureIntro. by eapply len_varray.
+  Qed.
+    
+  Definition op_safe op (i j: nat) : Prop :=
+    Z.to_nat (Int.intval (op (Int.repr i) (Int.repr j))) = i * j.
+
+  Definition mul_safe := op_safe Int.mul.
+
+  Lemma app_cons {A} (x: A) (y: list A):
+    [x] ++ y = x::y.
+  Proof. induction y; crush. Qed.
+  
+  Lemma index_spec q t p (i n: nat) vs Φ:
+    i < n → mul_safe (sizeof_type t) i →
     p ↦{q} varray vs @ tyarray t n ∗ (∀ v, p ↦{q} varray vs @ tyarray t n -∗ ⌜ vs !! i = Some v⌝ -∗ Φ v)
     ⊢ WP !(index t p (Int.repr i))@t {{ Φ }}.
   Proof.
-    iIntros (?) "[Hp HΦ]". destruct p.
+    iIntros (??) "[Hp HΦ]". destruct p.
     iDestruct (array_slice' with "Hp") as "Hs".
     destruct i.
     - unfold index. wp_op.
@@ -168,20 +207,50 @@ Section array.
       simpl. iDestruct (array_slice with "~") as "?".
       rewrite Nat.mul_1_r. done.
     - unfold index. wp_op.
-      wp_op. rewrite /offset_by_int32.
-      replace (Z.to_nat (Int.intval (Int.mul (Int.repr (sizeof_type t))
-                (Int.repr (Z.pos (Pos.of_succ_nat i))))))%nat with (sizeof_type t * S i).
-      iDestruct (split_slice _ _ b o (S i) 0 (n - S i)
-                             (take (S i) vs) (drop (S i) vs)
-                 with "[Hs]") as "[? ?]".
-      { admit. }
+      wp_op. rewrite /offset_by_int32. rewrite H1.
+      iDestruct (len_slice with "Hs") as "%".
+      iDestruct (split_slice' _ _ b o (S i) n vs with "[Hs]") as "[? ?]"=>//.
       simpl. destruct (n - S i) eqn:?.
-      { admit. }
+      { exfalso. omega. }
       destruct (drop (S i) vs) eqn:?.
-      { admit. }
+      { exfalso. assert (length (drop (S i) vs) = 0).
+        { by rewrite Heql. }
+        rewrite drop_length in H3. rewrite H2 in H3.
+        omega.
+      }
       simpl. iDestruct "~1" as "[? ?]".
       wp_load. iApply wp_value=>//.
       iApply ("HΦ" with "[-]").
-  Admitted.
+      + iApply array_slice'.
+        iDestruct (single_slice with "~1") as "Hm".
+        destruct (take (S i) vs) eqn:?.
+        { by iDestruct "~" as "%". }
+        iDestruct "~" as "[H1 H2]".
+        iDestruct (single_slice with "H1") as "H0".
+        (* XX: I should really write a super awesome framing tactic ... *)
+        assert (1 = 0 + 1) as Hi; first omega.
+        rewrite {1}Hi.
+        iDestruct (split_slice_join with "[H2 H0]") as "?"; first iFrame.
+        replace (1 + i) with (S i); last omega.
+        assert (S i = 0 + S i); first omega.
+        rewrite {2}H3.
+        iDestruct (split_slice_join with "[Hm ~]") as "?"; first iFrame.
+        replace (S (S i)) with (0 + (S i + 1)); last omega.
+        iDestruct (split_slice_join with "[-]") as "?"; first iFrame.
+        replace (S i + 1 + n0) with n; last omega.
+        replace ((([v0] ++ l0) ++ [v]) ++ l) with vs=>//.
+        rewrite -assoc.
+        rewrite !app_cons. rewrite -Heql -Heql0.
+        by rewrite take_drop.
+      + destruct (vs !! S i) eqn:?.
+        * iPureIntro. f_equal.
+          move:(take_drop_middle _ _ _ Heqo0)=>H3.
+          rewrite -H3 in Heql.
+          rewrite take_drop_app in Heql=>//.
+          { by inversion Heql. }
+          rewrite H2. omega.
+        * rewrite -H2 in H0. apply lookup_lt_is_Some in H0.
+          iPureIntro. inversion H0. rewrite H3 in Heqo0. done.
+  Qed.
 
 End array.
